(rocq-checker) reorganize transitions and steps to match the C implementation

src/casemate-check-rocq/src/casemate.ml
@@ -18,13 +18,13 @@ let parse_line line =
   let prefix = "\o033[46;37;1m" and suffix = "\o033[0m" in
   match strip_prefix line ~prefix with
   | None -> None
-  | Some line' ->
+  | Some line' -> (
       match strip_suffix line' ~suffix with
       | None -> Fmt.invalid_arg "Ill-formed line: %S" line
-      | Some line' ->
+      | Some line' -> (
           match Parser.of_line line' with
           | None -> Fmt.invalid_arg "Parse error: %S" line
-          | res -> res
+          | res -> res))
 
 let transitions ic = Iters.lines ic |> Iters.filter_map parse_line
 
@@ -60,17 +60,17 @@ let run_model ?(dump_state = false) ?(dump_roots = false) ?(dump_trans = false)
   let xs = match limit with Some n -> Iters.take n xs | _ -> xs in
   let step_ state trans =
     let res = Coq_executable_sm.take_step trans state in
-    if res.gsmsr_log != [] then (
+    if res.cmr_log != [] then (
       if dump_trans then
-        Fmt.pr "%a@ @[<2>%a@]@." pp_tr trans pp_logs res.gsmsr_log
-      else Fmt.pr "%a@." pp_logs res.gsmsr_log;
+        Fmt.pr "%a@ @[<2>%a@]@." pp_tr trans pp_logs res.cmr_log
+      else Fmt.pr "%a@." pp_logs res.cmr_log;
       if dump_roots then
-        Fmt.pr "@[<2>Roots:@ @[<2>%a@]@]@." pp_pte_roots state.gsm_roots;
+        Fmt.pr "@[<2>Roots:@ @[<2>%a@]@]@." pp_pte_roots state.cm_roots;
       if dump_state then
         Fmt.pr "@[<2>State:@ @[<2>%a@]@]@." pp_casemate_model state);
     (* If we reach an error, we dump the transition *)
-    if Result.is_error res.gsmsr_data then Fmt.pr "@[%a@]@." pp_tr trans;
-    res.gsmsr_data
+    if Result.is_error res.cmr_data then Fmt.pr "@[%a@]@." pp_tr trans;
+    res.cmr_data
   in
   Iters.fold_result step_ memory_init xs |> Fmt.pr "@[%a@]@." pp_step_result
 
