src/casemate-check-rocq/src/parser.ml
@@ -3,22 +3,23 @@ open Sexplib0.Sexp
 open Sexplib0.Sexp_conv
 open Coq_executable_sm
 
-let (~$) = Z0.(~$)
-
+let ( ~$ ) = Z0.( ~$ )
 let int = Sexplib0.Sexp_conv.int_of_sexp
-let u64 sexp = match sexp with
-| List _ -> of_sexp_error "bad u64" sexp
-| Atom s ->
-    let n = String.length s in
-    try (
-      if n > 2 && s.[0] == '0' && s.[1] == 'x' then
-        Z0.of_substring_base 16 s ~pos:2 ~len:(n - 2)
-      else Z0.of_string s
-    ) with Invalid_argument _ -> of_sexp_error "bad u64" sexp
+
+let u64 sexp =
+  match sexp with
+  | List _ -> of_sexp_error "bad u64" sexp
+  | Atom s -> (
+      let n = String.length s in
+      try
+        if n > 2 && s.[0] == '0' && s.[1] == 'x' then
+          Z0.of_substring_base 16 s ~pos:2 ~len:(n - 2)
+        else Z0.of_string s
+      with Invalid_argument _ -> of_sexp_error "bad u64" sexp)
 
 let mem_write_order = function
-  | Atom "plain"   -> WMO_plain
-  | Atom "page"    -> WMO_page
+  | Atom "plain" -> WMO_plain
+  | Atom "page" -> WMO_page
   | Atom "release" -> WMO_release
   | sexp -> of_sexp_error "bad mem-write mem-order" sexp
 
@@ -28,135 +29,219 @@ let msr_sysreg = function
   | sexp -> of_sexp_error "bad msr sysreg" sexp
 
 let hint_kind = function
-  | Atom "set_root_lock"        -> GHOST_HINT_SET_ROOT_LOCK
-  | Atom "set_owner_root"       -> GHOST_HINT_SET_OWNER_ROOT
-  | Atom "release_table"        -> GHOST_HINT_RELEASE
+  | Atom "set_root_lock" -> GHOST_HINT_SET_ROOT_LOCK
+  | Atom "set_owner_root" -> GHOST_HINT_SET_OWNER_ROOT
+  | Atom "release" -> GHOST_HINT_RELEASE_TABLE
   | Atom "set_pte_thread_owner" -> GHOST_HINT_SET_PTE_THREAD_OWNER
   | sexp -> of_sexp_error "bad lock hint kind" sexp
 
 let barrier_kind = function
-  | Atom "ish"   -> MBReqDomain_InnerShareable
+  | Atom "ish" -> MBReqDomain_InnerShareable
   | Atom "ishst" -> MBReqDomain_InnerShareable
-  | Atom "nsh"   -> MBReqDomain_Nonshareable
-  | Atom "sy"    -> MBReqDomain_FullSystem
-  | sexp         -> of_sexp_error "bad barrier kind" sexp
+  | Atom "nsh" -> MBReqDomain_Nonshareable
+  | Atom "sy" -> MBReqDomain_FullSystem
+  | sexp -> of_sexp_error "bad barrier kind" sexp
+
+let barrier_of = function
+  | List [ Atom "dsb"; List [ Atom "kind"; kind ] ] ->
+      Barrier_DSB (barrier_kind kind)
+  | Atom "isb" -> Barrier_ISB ()
+  | sexp -> of_sexp_error "bad barrier" sexp
 
 let tlbi_op = function
-| `DALL     -> TLBIOp_DALL        
-| `DASID    -> TLBIOp_DASID       
-| `DVA      -> TLBIOp_DVA         
-| `IALL     -> TLBIOp_IALL        
-| `IASID    -> TLBIOp_IASID       
-| `IVA      -> TLBIOp_IVA         
-| `ALL      -> TLBIOp_ALL         
-| `ASID     -> TLBIOp_ASID        
-| `IPAS2    -> TLBIOp_IPAS2       
-| `VAA      -> TLBIOp_VAA         
-| `VA       -> TLBIOp_VA          
-| `VMALL    -> TLBIOp_VMALL       
-| `VMALLS12 -> TLBIOp_VMALLS12    
-| `RIPAS2   -> TLBIOp_RIPAS2      
-| `RVAA     -> TLBIOp_RVAA        
-| `RVA      -> TLBIOp_RVA         
-| `RPA      -> TLBIOp_RPA         
-| `PAALL    -> TLBIOp_PAALL       
+  | `DALL -> TLBIOp_DALL
+  | `DASID -> TLBIOp_DASID
+  | `DVA -> TLBIOp_DVA
+  | `IALL -> TLBIOp_IALL
+  | `IASID -> TLBIOp_IASID
+  | `IVA -> TLBIOp_IVA
+  | `ALL -> TLBIOp_ALL
+  | `ASID -> TLBIOp_ASID
+  | `IPAS2 -> TLBIOp_IPAS2
+  | `VAA -> TLBIOp_VAA
+  | `VA -> TLBIOp_VA
+  | `VMALL -> TLBIOp_VMALL
+  | `VMALLS12 -> TLBIOp_VMALLS12
+  | `RIPAS2 -> TLBIOp_RIPAS2
+  | `RVAA -> TLBIOp_RVAA
+  | `RVA -> TLBIOp_RVA
+  | `RPA -> TLBIOp_RPA
+  | `PAALL -> TLBIOp_PAALL
+
 and regime_of = function
-| `EL3  -> Regime_EL3   
-| `EL30 -> Regime_EL30  
-| `EL2  -> Regime_EL2   
-| `EL20 -> Regime_EL20  
-| `EL10 -> Regime_EL10
+  | `EL3 -> Regime_EL3
+  | `EL30 -> Regime_EL30
+  | `EL2 -> Regime_EL2
+  | `EL20 -> Regime_EL20
+  | `EL10 -> Regime_EL10
+
 and shareability = function
-| `NSH -> Shareability_NSH
-| `ISH -> Shareability_ISH
-| `OSH -> Shareability_OSH
-and of_level sexp = match int sexp with
-| 0 | 1 | 2 -> TLBILevel_Any
-| 3 -> TLBILevel_Last
-| _ -> of_sexp_error "bad level" sexp
+  | `NSH -> Shareability_NSH
+  | `ISH -> Shareability_ISH
+  | `OSH -> Shareability_OSH
 
 let tlbi ?level ?addr ~regime ~shr op =
-  let level = match level with Some i -> of_level i | _ -> TLBILevel_Any
-  and address = match addr with Some a -> u64 a | _ -> Z0.zero
-  in {
+  let level =
+    match level with
+    | None -> TLBILevel_Any
+    | Some (Atom "any") -> TLBILevel_Any
+    | Some (Atom "last") -> TLBILevel_Last
+    | Some sexp -> of_sexp_error "bad tlbi level" sexp
+  and address = match addr with Some a -> u64 a | _ -> Z0.zero in
+  {
     tLBI_shareability = shareability shr;
-    tLBI_rec = {
-      tLBIRecord_op      = tlbi_op op;
-      tLBIRecord_regime  = regime_of regime;
-      tLBIRecord_level   = level;
-      tLBIRecord_address = address };
+    tLBI_rec =
+      {
+        tLBIRecord_op = tlbi_op op;
+        tLBIRecord_regime = regime_of regime;
+        tLBIRecord_level = level;
+        tLBIRecord_address = address;
+      };
   }
 
-let tlbi_of kind addr level sexp0 = match kind, addr, level with
-| "vmalls12e1",   None,      None -> tlbi `VMALLS12 ~regime:`EL10 ~shr:`NSH
-| "vmalls12e1is", None,      None -> tlbi `VMALLS12 ~regime:`EL10 ~shr:`ISH
-| "vmalle1is",    None,      None -> tlbi `VMALL    ~regime:`EL10 ~shr:`ISH
-| "alle1is",      None,      None -> tlbi `ALL      ~regime:`EL10 ~shr:`ISH
-| "vmalle1",      None,      None -> tlbi `VMALL    ~regime:`EL10 ~shr:`NSH (* XXX ? *)
-| "vae2is",       Some addr, Some level -> tlbi `VA ~regime:`EL2 ~shr:`ISH ~addr ~level
-| "ipas2e1is",    Some addr, Some level -> tlbi `IPAS2 ~regime:`EL10 ~shr:`NSH ~addr ~level
-| "vale2is",      Some addr, Some level -> tlbi `VA ~regime:`EL2 ~shr:`ISH ~addr ~level
-| _ -> of_sexp_error "bad tlbi" sexp0
+let tlbi_of = function
+  | Atom "vmalls12e1" -> tlbi `VMALLS12 ~regime:`EL10 ~shr:`NSH
+  | Atom "vmalls12e1is" -> tlbi `VMALLS12 ~regime:`EL10 ~shr:`ISH
+  | Atom "vmalle1is" -> tlbi `VMALL ~regime:`EL10 ~shr:`ISH
+  | Atom "alle1is" -> tlbi `ALL ~regime:`EL10 ~shr:`ISH
+  | List
+      [ Atom "vae2"; List [ Atom "addr"; addr ]; List [ Atom "level"; level ] ]
+    ->
+      tlbi `VA ~regime:`EL2 ~shr:`NSH ~addr ~level
+  | List
+      [
+        Atom "vae2is"; List [ Atom "addr"; addr ]; List [ Atom "level"; level ];
+      ] ->
+      tlbi `VA ~regime:`EL2 ~shr:`ISH ~addr ~level
+  | List
+      [
+        Atom "ipas2e1is";
+        List [ Atom "addr"; addr ];
+        List [ Atom "level"; level ];
+      ] ->
+      tlbi `IPAS2 ~regime:`EL10 ~shr:`NSH ~addr ~level
+  | sexp -> of_sexp_error "bad tlbi" sexp
 
 let transition sexp =
-  let data, id, tid, tl = match sexp with
-  | List (Atom "mem-write" :: id :: tid ::
-        List [Atom "mem-order"; o] :: List [Atom "address"; a] :: List [Atom "value"; v] :: tl) ->
-      GSMDT_TRANS_MEM_WRITE { twd_mo = mem_write_order o; twd_phys_addr = u64 a; twd_val = u64 v },
-      id, tid, tl
-  | List (Atom "mem-set" :: id :: tid::
-        List [Atom "address"; a] :: List [Atom "size"; s] :: List [Atom "value"; v] :: tl) ->
-      if u64 s <> ~$4096 then of_sexp_error "bad mem-set size" sexp else
-      GSMDT_TRANS_MEM_WRITE { twd_mo = WMO_page; twd_phys_addr = u64 a; twd_val = u64 v },
-      id, tid, tl
-  | List (Atom "mem-read" :: id :: tid::
-        List [Atom "address"; a] :: List [Atom "value"; v] :: tl) ->
-      GSMDT_TRANS_MEM_READ { trd_phys_addr = u64 a; trd_val = u64 v },
-      id, tid, tl
-  | List (Atom "mem-init" :: id :: tid::
-        List [Atom "address"; a] :: List [Atom "size"; s] :: tl) ->
-      GSMDT_TRANS_MEM_ZALLOC { tzd_addr = u64 a; tzd_size = u64 s },
-      id, tid, tl
-  | List (Atom "barrier" :: id :: tid :: Atom "isb" :: tl) ->
-      GSMDT_TRANS_BARRIER (Barrier_ISB ()), id, tid, tl
-  | List (Atom "barrier" :: id :: tid :: Atom "dsb" :: List [Atom "kind"; kind] :: tl) ->
-      GSMDT_TRANS_BARRIER (Barrier_DSB (barrier_kind kind)), id, tid, tl
-  | List (Atom "tlbi" :: id :: tid::
-        Atom kind :: List [Atom "addr"; a] :: List [Atom "level"; level] :: tl) ->
-      GSMDT_TRANS_TLBI (tlbi_of kind (Some a) (Some level) sexp), id, tid, tl
-  | List (Atom "tlbi" :: id :: tid:: Atom kind :: tl) ->
-      GSMDT_TRANS_TLBI (tlbi_of kind None None sexp), id, tid, tl
-  | List (Atom "sysreg-write" :: id :: tid::
-        List [Atom "sysreg"; sysreg] :: List [Atom "value"; v] :: tl) ->
-      GSMDT_TRANS_MSR { tmd_sysreg = msr_sysreg sysreg; tmd_val = u64 v },
-      id, tid, tl
-  | List (Atom "hint" :: id :: tid::
-        List [Atom "kind"; kind] :: List [Atom "location"; loc] :: List [Atom "value"; v] :: tl) ->
-      GSMDT_TRANS_HINT { thd_hint_kind = hint_kind kind; thd_location = u64 loc; thd_value = u64 v },
-      id, tid, tl
-  | List (Atom "lock" :: id :: tid :: List [Atom "address"; a] :: tl) ->
-      GSMDT_TRANS_LOCK { tld_kind = LOCK; tld_addr = u64 a }, id, tid, tl
-  | List (Atom "unlock" :: id :: tid :: List [Atom "address"; a] :: tl) ->
-      GSMDT_TRANS_LOCK { tld_kind = UNLOCK; tld_addr = u64 a }, id, tid, tl
-  | sexp -> of_sexp_error "bad event" sexp
+  let data, id, tid, tl =
+    match sexp with
+    | List
+        (Atom "mem-write"
+        :: id :: tid
+        :: List [ Atom "mem-order"; order ]
+        :: List [ Atom "address"; addr ]
+        :: List [ Atom "value"; value ]
+        :: tl) ->
+        ( CMSD_TRANS_HW_MEM_WRITE
+            {
+              twd_mo = mem_write_order order;
+              twd_phys_addr = u64 addr;
+              twd_val = u64 value;
+            },
+          id,
+          tid,
+          tl )
+    (*| List*)
+    (*    (Atom "mem-set"*)
+    (*    :: id :: tid*)
+    (*    :: List [ Atom "address"; addr ]*)
+    (*    :: List [ Atom "size"; size ]*)
+    (*    :: List [ Atom "value"; value ]*)
+    (*    :: tl) ->*)
+    (*    if u64 size <> ~$4096 then of_sexp_error "bad mem-set size" sexp*)
+    (*    else*)
+    (*      ( CMSD_TRANS_HW_MEM_WRITE*)
+    (*          {*)
+    (*            twd_mo = WMO_page;*)
+    (*            twd_phys_addr = u64 addr;*)
+    (*            twd_val = u64 value;*)
+    (*          },*)
+    (*        id,*)
+    (*        tid,*)
+    (*        tl )*)
+    | List
+        (Atom "mem-read"
+        :: id :: tid
+        :: List [ Atom "address"; addr ]
+        :: List [ Atom "value"; value ]
+        :: tl) ->
+        ( CMSD_TRANS_HW_MEM_READ
+            { trd_phys_addr = u64 addr; trd_val = u64 value },
+          id,
+          tid,
+          tl )
+    | List (Atom "barrier" :: id :: tid :: barrier :: tl) ->
+        (CMSD_TRANS_HW_BARRIER (barrier_of barrier), id, tid, tl)
+    | List (Atom "tlbi" :: id :: tid :: tlbi :: tl) ->
+        (CMSD_TRANS_HW_TLBI (tlbi_of tlbi), id, tid, tl)
+    | List
+        (Atom "sysreg-write"
+        :: id :: tid
+        :: List [ Atom "sysreg"; sysreg ]
+        :: List [ Atom "value"; value ]
+        :: tl) ->
+        ( CMSD_TRANS_HW_MSR
+            { tmd_sysreg = msr_sysreg sysreg; tmd_val = u64 value },
+          id,
+          tid,
+          tl )
+    | List
+        (Atom "mem-init"
+        :: id :: tid
+        :: List [ Atom "address"; addr ]
+        :: List [ Atom "size"; size ]
+        :: tl) ->
+        ( CMSD_TRANS_ABS_MEM_INIT { tid_addr = u64 addr; tid_size = u64 size },
+          id,
+          tid,
+          tl )
+    | List
+        (Atom "mem-set"
+        :: id :: tid
+        :: List [ Atom "address"; addr ]
+        :: List [ Atom "size"; size ]
+        :: List [ Atom "value"; value ]
+        :: tl) ->
+        ( CMSD_TRANS_ABS_MEMSET
+            { tmd_addr = u64 addr; tmd_size = u64 size; tmd_value = u64 value },
+          id,
+          tid,
+          tl )
+    | List (Atom "lock" :: id :: tid :: List [ Atom "address"; addr ] :: tl) ->
+        (CMSD_TRANS_ABS_LOCK (u64 addr), id, tid, tl)
+    | List (Atom "unlock" :: id :: tid :: List [ Atom "address"; addr ] :: tl)
+      ->
+        (CMSD_TRANS_ABS_UNLOCK (u64 addr), id, tid, tl)
+    | List
+        (Atom "hint"
+        :: id :: tid
+        :: List [ Atom "kind"; kind ]
+        :: List [ Atom "location"; loc ]
+        :: List [ Atom "value"; value ]
+        :: tl) ->
+        ( CMSD_TRANS_HINT
+            {
+              thd_hint_kind = hint_kind kind;
+              thd_location = u64 loc;
+              thd_value = u64 value;
+            },
+          id,
+          tid,
+          tl )
+    | sexp -> of_sexp_error "bad event" sexp
   in
-  let id = match id with
-    | List [Atom "id"; id] -> int id
-    | sexp -> of_sexp_error "bad id" sexp
-  and tid = match tid with
-    | List [Atom "tid"; tid] -> int tid
-    | sexp -> of_sexp_error "bad tid" sexp
-  and loc = match tl with
-    | [List [Atom "src"; Atom _loc]] -> None
+  let loc =
+    match tl with
+    | [ List [ Atom "src"; Atom _loc ] ] -> None
     | [] -> None
     | sexp -> of_sexp_error "bad location or extra data" (List sexp)
   in
-  Some {
-    gsmt_src_loc = loc;
-    gsmt_id = id;
-    gsmt_thread_identifier = tid;
-    gsmt_data = data
-  }
+  Some
+    {
+      cms_src_loc = loc;
+      cms_id = int id;
+      cms_thread_identifier = int tid;
+      cms_data = data;
+    }
 
 let of_line line = Sexplib.Sexp.of_string_conv_exn line transition
-
