src/casemate-check-rocq/theories/step.v
@@ -14,17 +14,17 @@ Require Export transition.
 
 (** Write *)
 
-(* Visiting a page table fails with this visitor iff the visited part has an uninitialized or invalid unclean entry *)
+(* Visiting a page table fails with this visitor iff the visited part has an uninitialised or invalid unclean entry *)
 Definition clean_reachable_cb (ctx : page_table_context) : casemate_model_result :=
   match ctx.(ptc_loc) with
-    | None => Merror (GSME_uninitialised "clean_reachable" ctx.(ptc_addr))
+    | None => Merror (CME_uninitialised "clean_reachable" ctx.(ptc_addr))
     | Some location =>
       match location.(sl_pte) with
         | None => Mreturn ctx.(ptc_state)
         | Some descriptor =>
           match descriptor.(ged_state) with
             | SPS_STATE_PTE_INVALID_UNCLEAN _ =>
-              Merror (GSME_unclean_child ctx.(ptc_addr))
+              Merror (CME_unclean_child ctx.(ptc_addr))
             | _ => Mreturn ctx.(ptc_state)
           end
       end
@@ -34,7 +34,7 @@ Definition clean_reachable_cb (ctx : page_table_context) : casemate_model_result
 Definition clean_reachable
   (map : table_data_t)
   (descriptor : ghost_exploded_descriptor)
-  (gsm : casemate_model):
+  (cm : casemate_model):
   casemate_model_result :=
   traverse_pgt_from
     descriptor.(ged_owner)
@@ -43,7 +43,7 @@ Definition clean_reachable
     (next_level descriptor.(ged_level))
     descriptor.(ged_stage)
     clean_reachable_cb
-    gsm
+    cm
 .
 
 Definition step_write_table_mark_children
@@ -53,13 +53,13 @@ Definition step_write_table_mark_children
   (val : u64)
   (descriptor : ghost_exploded_descriptor)
   (visitor_cb : page_table_context -> casemate_model_result)
-  (gsm : casemate_model) :
+  (cm : casemate_model) :
   casemate_model_result :=
   if is_desc_valid val then
     (* Tests if the page table is well formed *)
     match descriptor.(ged_pte_kind) with
       | PTER_PTE_KIND_TABLE map =>
-        let st := clean_reachable map descriptor gsm in
+        let st := clean_reachable map descriptor cm in
         let st := Mlog
           (Log "BBM: invalid clean->valid"%string (phys_addr_val loc.(sl_phys_addr))) st in
         Mupdate_state (traverse_pgt_from
@@ -70,11 +70,11 @@ Definition step_write_table_mark_children
                           descriptor.(ged_stage)
                           visitor_cb) st
       | _ => Mlog
-            (Log "BBM: invalid clean->valid"%string (phys_addr_val loc.(sl_phys_addr))) (Mreturn gsm)
+            (Log "BBM: invalid clean->valid"%string (phys_addr_val loc.(sl_phys_addr))) (Mreturn cm)
     end
   else
     (* if the descriptor is invalid, do nothing *)
-    Mreturn gsm
+    Mreturn cm
 .
 
 Definition step_write_on_invalid
@@ -82,12 +82,12 @@ Definition step_write_on_invalid
   (wmo : write_memory_order)
   (loc : sm_location)
   (val : u64)
-  (gsm : casemate_model) :
+  (cm : casemate_model) :
   casemate_model_result :=
   (* If the location is a PTE table, tests if its children are clean *)
   match loc.(sl_pte) with
     | None => (* This should not happen because if we write on invalid, we write on PTE *)
-      Merror (GSME_internal_error IET_unexpected_none)
+      Merror (CME_internal_error IET_unexpected_none)
     | Some descriptor =>
       let descriptor := deconstruct_pte
           tid
@@ -96,8 +96,8 @@ Definition step_write_on_invalid
           descriptor.(ged_owner)
           descriptor.(ged_stage) in
       let new_loc := loc <| sl_val := val |> <| sl_pte := Some descriptor |> in
-      let new_gsm := gsm <| gsm_memory := <[ loc.(sl_phys_addr) := new_loc ]> gsm.(gsm_memory) |> in
-      step_write_table_mark_children tid wmo loc val descriptor (mark_cb tid) new_gsm
+      let new_cm := cm <| cm_memory := <[ loc.(sl_phys_addr) := new_loc ]> cm.(cm_memory) |> in
+      step_write_table_mark_children tid wmo loc val descriptor (mark_cb tid) new_cm
     end
 .
 
@@ -106,13 +106,13 @@ Definition step_write_on_invalid_unclean
   (wmo : write_memory_order)
   (loc : sm_location)
   (val : u64)
-  (gsm : casemate_model) :
+  (cm : casemate_model) :
   casemate_model_result :=
   (* Only invalid descriptor are allowed *)
   if is_desc_valid val then
-    (Merror (GSME_bbm_violation VT_valid_on_invalid_unclean loc.(sl_phys_addr)))
+    (Merror (CME_bbm_violation VT_valid_on_invalid_unclean loc.(sl_phys_addr)))
   else
-    Mreturn (gsm <|gsm_memory := <[loc.(sl_phys_addr) := loc <|sl_val := val|> ]> gsm.(gsm_memory) |>)
+    Mreturn (cm <|cm_memory := <[loc.(sl_phys_addr) := loc <|sl_val := val|> ]> cm.(cm_memory) |>)
 .
 
 Definition is_only_update_to_sw_bit (old new : u64) : bool :=
@@ -125,18 +125,18 @@ Definition require_bbm
   (val : u64) :
   option bool :=
   match loc.(sl_pte) with
-    | None => None (* PTE cannot be valid if it is not a PTE *)
-    | Some old_descriptor =>
-      let new_descriptor := deconstruct_pte tid old_descriptor.(ged_ia_region).(range_start) val old_descriptor.(ged_level) old_descriptor.(ged_owner) old_descriptor.(ged_stage) in
-      match old_descriptor.(ged_pte_kind), new_descriptor.(ged_pte_kind) with
-        | PTER_PTE_KIND_INVALID, _ | _, PTER_PTE_KIND_INVALID => Some false
-        | PTER_PTE_KIND_TABLE _, _ | _, PTER_PTE_KIND_TABLE _ => Some true
-        | PTER_PTE_KIND_MAP r1, PTER_PTE_KIND_MAP r2 =>
-          if negb (phys_addr_val r1.(oa_region).(range_size) b=? phys_addr_val r2.(oa_region).(range_size)) then
-            Some true
-          else
-            Some (negb (is_only_update_to_sw_bit loc.(sl_val) val))
-      end
+  | None => None (* PTE cannot be valid if it is not a PTE *)
+  | Some old_descriptor =>
+    let new_descriptor := deconstruct_pte tid old_descriptor.(ged_ia_region).(range_start) val old_descriptor.(ged_level) old_descriptor.(ged_owner) old_descriptor.(ged_stage) in
+    match old_descriptor.(ged_pte_kind), new_descriptor.(ged_pte_kind) with
+    | PTER_PTE_KIND_INVALID, _ | _, PTER_PTE_KIND_INVALID => Some false
+    | PTER_PTE_KIND_TABLE _, _ | _, PTER_PTE_KIND_TABLE _ => Some true
+    | PTER_PTE_KIND_MAP r1, PTER_PTE_KIND_MAP r2 =>
+      if negb (phys_addr_val r1.(oa_region).(range_size) b=? phys_addr_val r2.(oa_region).(range_size)) then
+        Some true
+      else
+        Some (negb (is_only_update_to_sw_bit loc.(sl_val) val))
+    end
   end
 .
 
@@ -145,23 +145,23 @@ Definition step_write_valid_on_valid
   (wmo : write_memory_order)
   (loc : sm_location)
   (val : u64)
-  (gsm : casemate_model) :
+  (cm : casemate_model) :
   casemate_model_result :=
   match require_bbm tid loc val with (* If no change in memory: no problem*)
-    | None => Merror (GSME_internal_error IET_unexpected_none)
-    | Some false =>
-        (* if the location des not require BBM, then we can update the value and the descriptor *)
-        match loc.(sl_pte) with
-          | None => (* This does not make sense because function is called on a pgt *)
-            Merror (GSME_internal_error IET_unexpected_none)
-          | Some pte =>
-            let new_pte := deconstruct_pte tid pte.(ged_ia_region).(range_start) val pte.(ged_level) pte.(ged_owner) pte.(ged_stage) in
-            let loc := loc <| sl_val := val |> <| sl_pte := Some new_pte |> in
-            Mreturn (insert_location loc gsm)
-        end
-    | Some true =>
-      (* Changing the descriptor is illegal *)
-      Merror (GSME_bbm_violation VT_valid_on_valid loc.(sl_phys_addr))
+  | None => Merror (CME_internal_error IET_unexpected_none)
+  | Some false =>
+      (* if the location des not require BBM, then we can update the value and the descriptor *)
+      match loc.(sl_pte) with
+      | None => (* This does not make sense because function is called on a pgt *)
+        Merror (CME_internal_error IET_unexpected_none)
+      | Some pte =>
+        let new_pte := deconstruct_pte tid pte.(ged_ia_region).(range_start) val pte.(ged_level) pte.(ged_owner) pte.(ged_stage) in
+        let loc := loc <| sl_val := val |> <| sl_pte := Some new_pte |> in
+        Mreturn (insert_location loc cm)
+      end
+  | Some true =>
+    (* Changing the descriptor is illegal *)
+    Merror (CME_bbm_violation VT_valid_on_valid loc.(sl_phys_addr))
   end
 .
 
@@ -170,24 +170,24 @@ Definition step_write_invalid_on_valid
   (wmo : write_memory_order)
   (loc : sm_location)
   (val : u64)
-  (gsm : casemate_model) :
+  (cm : casemate_model) :
   casemate_model_result :=
   (* Invalidation of pgt: changing the state to invalid unclean unguarded *)
   let old := loc.(sl_val) in
   match loc.(sl_pte) with
   | None => (* This does not make sense because function is called on a pgt *)
-      Merror (GSME_internal_error IET_unexpected_none)
+      Merror (CME_internal_error IET_unexpected_none)
   | Some descriptor =>
     let new_desc := descriptor <| ged_state := (SPS_STATE_PTE_INVALID_UNCLEAN {| ai_invalidator_tid := tid; ai_old_valid_desc :=  old; ai_lis := LIS_unguarded; |}) |> in
-    let gsm := (gsm <| gsm_memory := (<[ loc.(sl_phys_addr) := loc <|sl_pte := Some (new_desc)|> <| sl_val := val |> ]> gsm.(gsm_memory))|> ) in
+    let cm := (cm <| cm_memory := (<[ loc.(sl_phys_addr) := loc <|sl_pte := Some (new_desc)|> <| sl_val := val |> ]> cm.(cm_memory))|> ) in
     Mlog (Log "BBM: valid->invalid_unclean"%string (phys_addr_val loc.(sl_phys_addr)))
     match descriptor.(ged_pte_kind) with
     | PTER_PTE_KIND_TABLE map =>
-      let res := clean_reachable map descriptor gsm in
+      let res := clean_reachable map descriptor cm in
       let res := Mlog (Log "invalidating a table descriptor"%string (phys_addr_val loc.(sl_phys_addr))) res in
       (* If it is well formed, mark its children as page tables, otherwise, return the same error *)
       Mupdate_state (step_write_table_mark_children tid wmo loc val descriptor (mark_not_writable_cb tid)) res
-    | _ => Mreturn gsm
+    | _ => Mreturn cm
     end
   end
 .
@@ -197,77 +197,77 @@ Definition step_write_on_valid
   (wmo : write_memory_order)
   (loc : sm_location)
   (val : u64)
-  (gsm : casemate_model) :
+  (cm : casemate_model) :
   casemate_model_result :=
   if is_desc_valid val
-    then step_write_valid_on_valid tid wmo loc val gsm
+    then step_write_valid_on_valid tid wmo loc val cm
   else
-    step_write_invalid_on_valid tid wmo loc val gsm
+    step_write_invalid_on_valid tid wmo loc val cm
 .
 
 Definition is_valid_state (st: sm_pte_state) : bool :=
   match st with
-    | SPS_STATE_PTE_VALID _ => true
-    | _ => false
+  | SPS_STATE_PTE_VALID _ => true
+  | _ => false
   end
 .
 
-Definition drop_write_authorisation_of_lock
+Definition drop_write_authorization_of_lock
   (cpu : thread_identifier)
   (addr : phys_addr_t)
   (wmo : write_memory_order)
   (descriptor : u64)
   (pte : ghost_exploded_descriptor)
-  (gsm : casemate_model) :
+  (cm : casemate_model) :
   casemate_model_result :=
-  match get_lock_of_owner pte.(ged_owner) gsm with
-  | None => Mreturn gsm
+  match get_lock_of_owner pte.(ged_owner) cm with
+  | None => Mreturn cm
   | Some addr_lock =>
-    match lookup addr_lock gsm.(gsm_lock_state) with
+    match lookup addr_lock cm.(cm_lock_state) with
     | Some lock_owner =>
       if bool_decide (lock_owner = cpu) then
         match wmo with
         | WMO_page | WMO_plain => (* check that the write is authorized, and then drop the authorization *)
-          match lookup addr_lock gsm.(gsm_lock_authorization) with
-          | None => Merror (GSME_internal_error IET_no_write_authorization)
-          | Some write_authorized => Mreturn (gsm <| gsm_lock_authorization := insert addr_lock write_unauthorized gsm.(gsm_lock_authorization)|>)
+          match lookup addr_lock cm.(cm_lock_authorization) with
+          | None => Merror (CME_internal_error IET_no_write_authorization)
+          | Some write_authorized => Mreturn (cm <| cm_lock_authorization := insert addr_lock write_unauthorized cm.(cm_lock_authorization)|>)
           | Some write_unauthorized =>
             if (is_desc_valid descriptor) || is_valid_state pte.(ged_state) then
-              Merror (GSME_write_without_authorization addr)
+              Merror (CME_write_without_authorization addr)
             else
-              Mreturn (gsm <| gsm_lock_authorization := insert addr_lock write_unauthorized gsm.(gsm_lock_authorization)|>)
+              Mreturn (cm <| cm_lock_authorization := insert addr_lock write_unauthorized cm.(cm_lock_authorization)|>)
           end
         | WMO_release => (* drop the authorization*)
-          Mreturn (gsm <| gsm_lock_authorization := insert addr_lock write_unauthorized gsm.(gsm_lock_authorization)|>)
+          Mreturn (cm <| cm_lock_authorization := insert addr_lock write_unauthorized cm.(cm_lock_authorization)|>)
         end
       else
-        Merror (GSME_transition_without_lock addr)
-    | None => Merror (GSME_transition_without_lock addr)
+        Merror (CME_transition_without_lock addr)
+    | None => Merror (CME_transition_without_lock addr)
     end
   end
 .
 
-Definition drop_write_authorisation
+Definition drop_write_authorization
   (tid : thread_identifier)
   (wd : trans_write_data)
-  (gsm : casemate_model) :
+  (cm : casemate_model) :
   casemate_model_result :=
   let wmo := wd.(twd_mo) in
   let val := wd.(twd_val) in
   let addr := wd.(twd_phys_addr) in
   if negb ((bv_and_64 (phys_addr_val addr) b7) b=? b0)
-    then Merror GSME_unaligned_write
+    then Merror CME_unaligned_write
   else
-    match gsm !! addr with
-    | None => Mreturn gsm
+    match cm !! addr with
+    | None => Mreturn cm
     | Some location =>
         match location.(sl_pte) with
-        | None => Mreturn gsm
+        | None => Mreturn cm
         | Some pte =>
-          if is_loc_thread_owned tid location gsm then
-            Mreturn gsm
+          if is_loc_thread_owned tid location cm then
+            Mreturn cm
           else
-            drop_write_authorisation_of_lock tid addr wmo val pte gsm
+            drop_write_authorization_of_lock tid addr wmo val pte cm
         end
     end
 .
@@ -275,14 +275,13 @@ Definition drop_write_authorisation
 Definition step_write_aux
   (tid : thread_identifier)
   (wd : trans_write_data)
-  (gsm : casemate_model) :
-  casemate_model_result :=
+  (cm : casemate_model) : casemate_model_result :=
   let wmo := wd.(twd_mo) in
   let val := wd.(twd_val) in
   let addr := wd.(twd_phys_addr) in
   if negb ((bv_and_64 (phys_addr_val addr) b7) b=? b0)
-    then Merror GSME_unaligned_write else
-  let new_st := drop_write_authorisation tid wd gsm in
+    then Merror CME_unaligned_write else
+  let new_st := drop_write_authorization tid wd cm in
   let write_update s :=
     match s !! addr with
     | Some (loc) =>
@@ -297,28 +296,28 @@ Definition step_write_aux
         | SPS_STATE_PTE_INVALID_UNCLEAN av =>
             (step_write_on_invalid_unclean tid wmo loc val s)
         | SPS_STATE_PTE_NOT_WRITABLE =>
-            (Merror (GSME_write_on_not_writable addr))
+            (Merror (CME_write_on_not_writable addr))
         end
       | None => (* If it is not a pte, we just update the value *)
         let new_loc := loc <| sl_val := val |> in
         {|
-          gsmsr_log := nil;
-          gsmsr_data :=
+          cmr_log := nil;
+          cmr_data :=
             Ok _ _ (
-              s <| gsm_memory := <[ addr := new_loc ]> s.(gsm_memory) |>
+              s <| cm_memory := <[ addr := new_loc ]> s.(cm_memory) |>
             );
         |}
       end
     | None =>
       (* If the location has not been written to, it is not a pgt, just save its value *)
-        let new_st := s <| gsm_memory :=
+        let new_st := s <| cm_memory :=
             <[ addr := {|
                 sl_phys_addr := addr;
                 sl_val := val;
                 sl_pte := None;
                 sl_thread_owner := None;
               |}
-            ]> s.(gsm_memory) |> in
+            ]> s.(cm_memory) |> in
                 Mreturn new_st
           end
   in
@@ -350,73 +349,82 @@ Proof. lia. Qed.
 Definition step_write
   (tid : thread_identifier)
   (wd : trans_write_data)
-  (gsm : casemate_model) :
-  casemate_model_result :=
+  (cm : casemate_model) : casemate_model_result :=
   match wd.(twd_mo) with
-    | WMO_plain | WMO_release => step_write_aux tid wd gsm
-    | WMO_page => step_write_page tid wd (Mreturn gsm) z512
+  | WMO_plain | WMO_release => step_write_aux tid wd cm
+  | WMO_page => step_write_page tid wd (Mreturn cm) z512
   end
 .
 
+(** Mem init *)
 
-(** Zalloc *)
-
-Definition step_zalloc_aux
+Definition step_init_aux
   (addr : phys_addr_t)
   (st : casemate_model_result) :
   casemate_model_result :=
-  let update s := {| gsmsr_log := nil; gsmsr_data := Ok _ _ (s <| gsm_zalloc := <[ addr := () ]> s.(gsm_zalloc) |>) |} in
+  let update s := {| cmr_log := nil; cmr_data := Ok _ _ (s <| cm_initialised := <[ addr := () ]> s.(cm_initialised) |>) |} in
   Mupdate_state update st
 .
 
-Definition _step_zalloc_step_size := Phys_addr (bv_shiftl_64 b1 (bv64.BV64 3)).
+Definition _step_init_step_size := Phys_addr (bv_shiftl_64 b1 (bv64.BV64 3)).
 
-Fixpoint step_zalloc_all
+Fixpoint step_init_all
   (addr : phys_addr_t)
   (st : casemate_model_result)
   (offs : phys_addr_t)
   (max : nat) :
   casemate_model_result :=
   match max with
-    | O => st
-    | S max =>
-      let st := step_zalloc_aux (addr pa+ offs) st in
-      step_zalloc_all addr st (offs pa+ (_step_zalloc_step_size)) max
+  | O => st
+  | S max =>
+    let st := step_init_aux (addr pa+ offs) st in
+    step_init_all addr st (offs pa+ (_step_init_step_size)) max
   end
 .
 
-Definition step_zalloc
-  (zd : trans_zalloc_data)
-  (gsm : casemate_model) :
+Definition step_init
+  (init_data : trans_init_data)
+  (cm : casemate_model) :
   casemate_model_result :=
-  step_zalloc_all (Phys_addr (bv_shiftr_64 (phys_addr_val zd.(tzd_addr)) (bv64.BV64 9))) {|gsmsr_log := nil; gsmsr_data := Ok _ _ gsm|} pa0 (to_nat zd.(tzd_size))
+  step_init_all (Phys_addr (bv_shiftr_64 (phys_addr_val init_data.(tid_addr)) (bv64.BV64 9))) {|cmr_log := nil; cmr_data := Ok _ _ cm|} pa0 (to_nat init_data.(tid_size))
 .
 
+Definition step_memset
+  (tid : thread_identifier)
+  (memset_data : trans_memset_data)
+  (cm : casemate_model) : casemate_model_result :=
+  let write_data := {|
+    twd_mo := WMO_plain;
+    twd_phys_addr := memset_data.(tmd_addr);
+    twd_val := memset_data.(tmd_value);
+  |} in
+  (* memset is a plain write *)
+  step_write_page tid write_data (Mreturn cm) (bv64.to_Z (bv_shiftr_64 memset_data.(tmd_size) b3)).
 
 (** Read *)
 
 Definition step_read
   (tid : thread_identifier)
   (rd : trans_read_data)
-  (gsm : casemate_model) :
+  (cm : casemate_model) :
   casemate_model_result :=
-  (* Test if the memory has been initialized (it might refuse acceptable executions, not sure if it is a good idea) and its content is consistent. *)
-  match gsm !! rd.(trd_phys_addr) with
-    | Some loc =>
-        if loc.(sl_val) b=? rd.(trd_val) then
-          Mreturn gsm
-        else
-          let new_loc := loc <| sl_val := rd.(trd_val) |> in
-          {| gsmsr_log :=
-              [Inconsistent_read loc.(sl_val) rd.(trd_val) rd.(trd_phys_addr)];
-             gsmsr_data := (Ok _ _ (gsm <| gsm_memory := <[rd.(trd_phys_addr) := new_loc ]> gsm.(gsm_memory) |>)) |}
-    | None =>
-        let loc := {| sl_phys_addr := rd.(trd_phys_addr); sl_val := rd.(trd_val); sl_pte := None; sl_thread_owner := Some tid |} in
-        let st := gsm <| gsm_memory := <[ rd.(trd_phys_addr) := loc ]> gsm.(gsm_memory) |> in
-        {| gsmsr_log :=
-            [Warning_read_write_non_allocd loc.(sl_phys_addr)];
-           gsmsr_data := Ok _ _ st
-        |}
+  (* Test if the memory has been initialised (it might refuse acceptable executions, not sure if it is a good idea) and its content is consistent. *)
+  match cm !! rd.(trd_phys_addr) with
+  | Some loc =>
+      if loc.(sl_val) b=? rd.(trd_val) then
+        Mreturn cm
+      else
+        let new_loc := loc <| sl_val := rd.(trd_val) |> in
+        {| cmr_log :=
+            [Inconsistent_read loc.(sl_val) rd.(trd_val) rd.(trd_phys_addr)];
+           cmr_data := (Ok _ _ (cm <| cm_memory := <[rd.(trd_phys_addr) := new_loc ]> cm.(cm_memory) |>)) |}
+  | None =>
+      let loc := {| sl_phys_addr := rd.(trd_phys_addr); sl_val := rd.(trd_val); sl_pte := None; sl_thread_owner := Some tid |} in
+      let st := cm <| cm_memory := <[ rd.(trd_phys_addr) := loc ]> cm.(cm_memory) |> in
+      {| cmr_log :=
+          [Warning_read_write_non_allocd loc.(sl_phys_addr)];
+         cmr_data := Ok _ _ st
+      |}
   end
 .
 
@@ -433,10 +441,10 @@ Definition dsb_invalid_unclean_unmark_children
     deconstruct_pte cpu_id ptc.(ptc_partial_ia) lis.(ai_old_valid_desc) ptc.(ptc_level) ptc.(ptc_root) ptc.(ptc_stage)
   in
   match desc.(ged_pte_kind) with
-    | PTER_PTE_KIND_TABLE map =>
-      (* The children are clean, and not writable, otherwise, it would catch fire *)
-      traverse_pgt_from desc.(ged_owner) map.(next_level_table_addr) desc.(ged_ia_region).(range_start) (next_level desc.(ged_level)) desc.(ged_stage) (unmark_cb cpu_id) st
-    | _ => {| gsmsr_log  := nil; gsmsr_data := Ok _ _ st |}
+  | PTER_PTE_KIND_TABLE map =>
+    (* The children are clean, and not writable, otherwise, it would catch fire *)
+    traverse_pgt_from desc.(ged_owner) map.(next_level_table_addr) desc.(ged_ia_region).(range_start) (next_level desc.(ged_level)) desc.(ged_stage) (unmark_cb cpu_id) st
+  | _ => {| cmr_log  := nil; cmr_data := Ok _ _ st |}
   end
 .
 
@@ -446,32 +454,32 @@ Definition new_pte_after_dsb
   (pte : ghost_exploded_descriptor)
   (kind : DxB) : ghost_exploded_descriptor :=
   match pte.(ged_state) with
-    | SPS_STATE_PTE_INVALID_UNCLEAN sst =>
-      (* DSB has an effect on invalid unclean state only *)
-      if negb (bool_decide (sst.(ai_invalidator_tid) = cpu_id)) then
-        pte (* If it is another CPU that did the invalidation, do noting*)
-      else
-        (* Otherwise, update the state invalid unclean sub-automaton *)
-        match sst.(ai_lis) with
-          | LIS_unguarded =>
-            pte <|ged_state := SPS_STATE_PTE_INVALID_UNCLEAN (sst <| ai_lis := LIS_dsbed |>) |>
-          | LIS_dsbed => pte
-          | LIS_dsb_tlbied =>
-            match kind.(DxB_domain) with
-              | MBReqDomain_InnerShareable | MBReqDomain_FullSystem =>
-                pte <| ged_state := SPS_STATE_PTE_INVALID_CLEAN {| aic_invalidator_tid := sst.(ai_invalidator_tid) |} |>
-                    <| ged_pte_kind := PTER_PTE_KIND_INVALID |>
-              | _ => pte
-            end
-          | LIS_dsb_tlbi_ipa =>
-              match kind.(DxB_domain) with
-                | MBReqDomain_InnerShareable | MBReqDomain_FullSystem =>
-                  pte <|ged_state := SPS_STATE_PTE_INVALID_UNCLEAN (sst <|ai_lis := LIS_dsb_tlbi_ipa_dsb |>) |>
-                | _ => pte
-              end
-          | _ => pte
+  | SPS_STATE_PTE_INVALID_UNCLEAN sst =>
+    (* DSB has an effect on invalid unclean state only *)
+    if negb (bool_decide (sst.(ai_invalidator_tid) = cpu_id)) then
+      pte (* If it is another CPU that did the invalidation, do noting*)
+    else
+      (* Otherwise, update the state invalid unclean sub-automaton *)
+      match sst.(ai_lis) with
+      | LIS_unguarded =>
+        pte <|ged_state := SPS_STATE_PTE_INVALID_UNCLEAN (sst <| ai_lis := LIS_dsbed |>) |>
+      | LIS_dsbed => pte
+      | LIS_dsb_tlbied =>
+        match kind.(DxB_domain) with
+        | MBReqDomain_InnerShareable | MBReqDomain_FullSystem =>
+          pte <| ged_state := SPS_STATE_PTE_INVALID_CLEAN {| aic_invalidator_tid := sst.(ai_invalidator_tid) |} |>
+              <| ged_pte_kind := PTER_PTE_KIND_INVALID |>
+        | _ => pte
         end
-    | _ => pte (* If not invalid unclean, then do nothing *)
+      | LIS_dsb_tlbi_ipa =>
+          match kind.(DxB_domain) with
+          | MBReqDomain_InnerShareable | MBReqDomain_FullSystem =>
+            pte <|ged_state := SPS_STATE_PTE_INVALID_UNCLEAN (sst <|ai_lis := LIS_dsb_tlbi_ipa_dsb |>) |>
+          | _ => pte
+          end
+      | _ => pte
+      end
+  | _ => pte (* If not invalid unclean, then do nothing *)
   end
 .
 
@@ -481,80 +489,80 @@ Definition dsb_visitor
   (ctx : page_table_context) :
   casemate_model_result :=
   match ctx.(ptc_loc) with
-    | None => (* This case is not explicitly excluded by the C code, but we cannot do anything in this case. *)
-      Merror (GSME_uninitialised "dsb_visitor"%string ctx.(ptc_addr))
-    | Some location =>
-      match location.(sl_pte) with
-        | None => Merror (GSME_not_a_pte "dsb_visitor" ctx.(ptc_addr))
-        | Some pte =>
-          let new_pte := new_pte_after_dsb cpu_id pte kind in
-          (* then update state and return *)
-          let new_loc := (location <| sl_pte := Some new_pte |>) in
-          let new_state := ctx.(ptc_state) <| gsm_memory := <[ location.(sl_phys_addr) := new_loc ]> ctx.(ptc_state).(gsm_memory) |> in
-          let log :=
-            match pte.(ged_state), new_pte.(ged_state) with
-              | SPS_STATE_PTE_INVALID_UNCLEAN _ , SPS_STATE_PTE_INVALID_CLEAN _ =>
-                Some (Log "BBM: invalid_unclean->invalid_clean"%string (phys_addr_val location.(sl_phys_addr)))
-              | SPS_STATE_PTE_INVALID_UNCLEAN {| ai_lis := LIS_unguarded|} , SPS_STATE_PTE_INVALID_UNCLEAN {| ai_lis := _|} =>
-                Some (Log "BBM: unguareded->dsbed"%string (phys_addr_val location.(sl_phys_addr)))
-              | SPS_STATE_PTE_INVALID_UNCLEAN {| ai_lis := LIS_dsb_tlbi_ipa|} , SPS_STATE_PTE_INVALID_UNCLEAN {| ai_lis := _|} =>
-                Some (Log "BBM: tlbied_ipa->tlbied_ipa_dsbed"%string (phys_addr_val location.(sl_phys_addr)))
-              | _, _ => None
-            end
-          in
-          let new_state :=
-            match pte.(ged_state), new_pte.(ged_state) with
-              | SPS_STATE_PTE_INVALID_UNCLEAN lis , SPS_STATE_PTE_INVALID_CLEAN _ =>
-                dsb_invalid_unclean_unmark_children cpu_id new_loc lis
-                    (ctx <| ptc_state := new_state |> <|ptc_loc := Some new_loc|>)
-              | _, _ => Mreturn new_state
-            end
-          in
-          match log with
-          | Some txt => Mlog txt new_state
-          | None => new_state
-          end
+  | None => (* This case is not explicitly excluded by the C code, but we cannot do anything in this case. *)
+    Merror (CME_uninitialised "dsb_visitor"%string ctx.(ptc_addr))
+  | Some location =>
+    match location.(sl_pte) with
+    | None => Merror (CME_not_a_pte "dsb_visitor" ctx.(ptc_addr))
+    | Some pte =>
+      let new_pte := new_pte_after_dsb cpu_id pte kind in
+      (* then update state and return *)
+      let new_loc := (location <| sl_pte := Some new_pte |>) in
+      let new_state := ctx.(ptc_state) <| cm_memory := <[ location.(sl_phys_addr) := new_loc ]> ctx.(ptc_state).(cm_memory) |> in
+      let log :=
+        match pte.(ged_state), new_pte.(ged_state) with
+        | SPS_STATE_PTE_INVALID_UNCLEAN _ , SPS_STATE_PTE_INVALID_CLEAN _ =>
+          Some (Log "BBM: invalid_unclean->invalid_clean"%string (phys_addr_val location.(sl_phys_addr)))
+        | SPS_STATE_PTE_INVALID_UNCLEAN {| ai_lis := LIS_unguarded|} , SPS_STATE_PTE_INVALID_UNCLEAN {| ai_lis := _|} =>
+          Some (Log "BBM: unguareded->dsbed"%string (phys_addr_val location.(sl_phys_addr)))
+        | SPS_STATE_PTE_INVALID_UNCLEAN {| ai_lis := LIS_dsb_tlbi_ipa|} , SPS_STATE_PTE_INVALID_UNCLEAN {| ai_lis := _|} =>
+          Some (Log "BBM: tlbied_ipa->tlbied_ipa_dsbed"%string (phys_addr_val location.(sl_phys_addr)))
+        | _, _ => None
+        end
+      in
+      let new_state :=
+        match pte.(ged_state), new_pte.(ged_state) with
+        | SPS_STATE_PTE_INVALID_UNCLEAN lis , SPS_STATE_PTE_INVALID_CLEAN _ =>
+          dsb_invalid_unclean_unmark_children cpu_id new_loc lis
+              (ctx <| ptc_state := new_state |> <|ptc_loc := Some new_loc|>)
+        | _, _ => Mreturn new_state
+        end
+      in
+      match log with
+      | Some txt => Mlog txt new_state
+      | None => new_state
       end
+    end
   end
 .
 
 Fixpoint reset_write_authorizations_aux
   (tid : thread_identifier)
   (roots: list owner_t)
-  (gsm : casemate_model) :
+  (cm : casemate_model) :
   casemate_model :=
   match roots with
-  | [] => gsm
+  | [] => cm
   | h :: q =>
-    match lookup (phys_addr_val (root_val h)) gsm.(gsm_lock_addr) with
+    match lookup (phys_addr_val (root_val h)) cm.(cm_lock_addr) with
     | Some lock_addr =>
       let new_st :=
-        match lookup lock_addr gsm.(gsm_lock_state) with
-        | None => gsm
+        match lookup lock_addr cm.(cm_lock_state) with
+        | None => cm
         | Some thread =>
           if bool_decide (thread = tid) then
-            (gsm <| gsm_lock_authorization :=
-                insert lock_addr write_authorized gsm.(gsm_lock_authorization) |>)
+            (cm <| cm_lock_authorization :=
+                insert lock_addr write_authorized cm.(cm_lock_authorization) |>)
           else
-            gsm
+            cm
         end
       in
       reset_write_authorizations_aux tid q new_st
-    | None => reset_write_authorizations_aux tid q gsm
+    | None => reset_write_authorizations_aux tid q cm
     end
   end
 .
 
 
-Definition reset_write_authorizations (tid : thread_identifier) (gsm : casemate_model) : casemate_model :=
+Definition reset_write_authorizations (tid : thread_identifier) (cm : casemate_model) : casemate_model :=
   (* Reset the authorizations for both states *)
-  reset_write_authorizations_aux tid gsm.(gsm_roots).(pr_s2)
-    (reset_write_authorizations_aux tid gsm.(gsm_roots).(pr_s1) gsm)
+  reset_write_authorizations_aux tid cm.(cm_roots).(pr_s2)
+    (reset_write_authorizations_aux tid cm.(cm_roots).(pr_s1) cm)
 .
 
-Definition step_dsb (tid : thread_identifier) (dk : DxB) (gsm : casemate_model) : casemate_model_result :=
+Definition step_dsb (tid : thread_identifier) (dk : DxB) (cm : casemate_model) : casemate_model_result :=
   (* There is enough barrier now to write plain again *)
-  let st := reset_write_authorizations tid gsm in
+  let st := reset_write_authorizations tid cm in
   (* walk the pgt with dsb_visitor*)
   traverse_all_pgt (Some tid) st (dsb_visitor dk tid)
 .
@@ -563,67 +571,67 @@ Definition step_dsb (tid : thread_identifier) (dk : DxB) (gsm : casemate_model) 
 
 Definition is_leaf (kind : pte_rec) : bool :=
   match kind with
-    | PTER_PTE_KIND_TABLE _ => false
-    | _ => true
+  | PTER_PTE_KIND_TABLE _ => false
+  | _ => true
   end
 .
 
 Definition is_last_level_only (d : TLBI_op_by_addr_data) : bool :=
   match d.(TOBAD_last_level_only) with
-    | TLBILevel_Any => false
-    | TLBILevel_Last => true
+  | TLBILevel_Any => false
+  | TLBILevel_Last => true
   end
 .
 
 Definition should_perform_tlbi (td : TLBI_intermediate) (ptc : page_table_context) : option bool :=
   match ptc.(ptc_loc) with
-    | None => None (* does not happen because we call it in tlbi_visitor in which we test that the location is init *)
-    | Some loc =>
-      match loc.(sl_pte) with
-        | None => None (* if the PTE is not initialised, it has not been used; TLBI has no effect *)
-        | Some pte_desc =>
-          match td.(TI_method) with
-            | TLBI_by_input_addr d =>
-              let tlbi_addr := bv_shiftl_64 (phys_addr_val d.(TOBAD_page)) b12 in
-              let ia_start := pte_desc.(ged_ia_region).(range_start) in
-              let ia_end := ia_start pa+ pte_desc.(ged_ia_region).(range_size) in
-              if (is_leaf pte_desc.(ged_pte_kind)
-                       && (phys_addr_val ia_start b<=? tlbi_addr)
-                       && (tlbi_addr b<? phys_addr_val ia_end)) then
-                Some false
-              else if ((negb (is_l3 pte_desc.(ged_level))) && is_last_level_only d) then
-                Some false
-              else
-                Some true
-            | TLBI_by_addr_space _ => None
-            | TLBI_by_addr_all => Some true
-          end
+  | None => None (* does not happen because we call it in tlbi_visitor in which we test that the location is init *)
+  | Some loc =>
+    match loc.(sl_pte) with
+    | None => None (* if the PTE is not initialised, it has not been used; TLBI has no effect *)
+    | Some pte_desc =>
+      match td.(TI_method) with
+      | TLBI_by_input_addr d =>
+        let tlbi_addr := bv_shiftl_64 (phys_addr_val d.(TOBAD_page)) b12 in
+        let ia_start := pte_desc.(ged_ia_region).(range_start) in
+        let ia_end := ia_start pa+ pte_desc.(ged_ia_region).(range_size) in
+        if (is_leaf pte_desc.(ged_pte_kind)
+                 && (phys_addr_val ia_start b<=? tlbi_addr)
+                 && (tlbi_addr b<? phys_addr_val ia_end)) then
+          Some false
+        else if ((negb (is_l3 pte_desc.(ged_level))) && is_last_level_only d) then
+          Some false
+        else
+          Some true
+      | TLBI_by_addr_space _ => None
+      | TLBI_by_addr_all => Some true
       end
+    end
   end
 .
 
 
 Definition step_pte_on_tlbi_after_dsb (td: TLBI_intermediate) : option LIS :=
   match td.(TI_regime) with
-    | Regime_EL2 => Some LIS_dsb_tlbied
-    | Regime_EL10 =>
-      match td.(TI_stage) with
-        | TLBI_OP_stage1 => Some LIS_dsbed (* no effect*)
-        | TLBI_OP_stage2 => Some LIS_dsb_tlbi_ipa
-        | TLBI_OP_both_stages => Some LIS_dsb_tlbied
-      end
-    | _ => None
+  | Regime_EL2 => Some LIS_dsb_tlbied
+  | Regime_EL10 =>
+    match td.(TI_stage) with
+    | TLBI_OP_stage1 => Some LIS_dsbed (* no effect*)
+    | TLBI_OP_stage2 => Some LIS_dsb_tlbi_ipa
+    | TLBI_OP_both_stages => Some LIS_dsb_tlbied
+    end
+  | _ => None
   end
 .
 
 Definition step_pte_on_tlbi_after_tlbi_ipa (td: TLBI_intermediate) : option LIS :=
   match td.(TI_regime) with
-    | Regime_EL10 =>
-        match td.(TI_stage) with
-          | TLBI_OP_stage1 | TLBI_OP_both_stages => Some LIS_dsb_tlbied
-          | TLBI_OP_stage2 => Some LIS_dsb_tlbi_ipa_dsb
-        end
-    | _ => None
+  | Regime_EL10 =>
+      match td.(TI_stage) with
+      | TLBI_OP_stage1 | TLBI_OP_both_stages => Some LIS_dsb_tlbied
+      | TLBI_OP_stage2 => Some LIS_dsb_tlbi_ipa_dsb
+      end
+  | _ => None
   end
 .
 
@@ -633,73 +641,73 @@ Definition tlbi_visitor
   (ptc : page_table_context) :
   casemate_model_result :=
   match ptc.(ptc_loc) with
-    | None => (* Cannot do anything if the page is not initialized *)
-      Merror (GSME_uninitialised "tlbi_visitor" ptc.(ptc_addr))
-    | Some location =>
-      (* Test if there is something to do *)
-      match should_perform_tlbi td ptc with
-        | None => Merror GSME_unimplemented
-        | Some b =>
-          if b then
-            (* step_pte_on_tlbi: inlined *)
-            match location.(sl_pte) with
-              | None => Merror (GSME_internal_error IET_unexpected_none)
-                (* This cannot happen (otherwise, should_perform_tlbi would be false) *)
-              | Some exploded_desc =>
-                match exploded_desc.(ged_state) with
-                  | SPS_STATE_PTE_INVALID_UNCLEAN ai =>
-                    (* If the CPU that does the transformation is not the one that initiated the invalidation, do nothing *)
-                    if bool_decide (cpu_id = ai.(ai_invalidator_tid)) then
-                      let new_substate :=
-                        (* Depending on the current state and the TLBI kind, we update the sub-state *)
-                        match ai.(ai_lis) with
-                          | LIS_dsbed => step_pte_on_tlbi_after_dsb td
-                          | LIS_dsb_tlbi_ipa_dsb => step_pte_on_tlbi_after_tlbi_ipa td
-                          | a => Some a (* Otherwise, it does not make the sub-automaton change *)
-                        end
-                      in
-                      match new_substate with
-                        | None => Merror GSME_unimplemented
-                        | Some new_substate =>
-                          let log :=
-                            match new_substate, ai.(ai_lis) with
-                              | LIS_dsb_tlbied, LIS_dsbed => Mlog (Log "BBM: dsb'd->tlbied" (phys_addr_val ptc.(ptc_addr)))
-                              | LIS_dsb_tlbi_ipa, LIS_dsbed => Mlog (Log "BBM: dsb'd->tlbied_ipa" (phys_addr_val ptc.(ptc_addr)))
-                              | LIS_dsb_tlbied, LIS_dsb_tlbi_ipa_dsb => Mlog (Log "BBM: dsb_tlbi_ipa_dsbed->tlbied" (phys_addr_val ptc.(ptc_addr)))
-                              | _, _ => id
-                            end
-                          in
-                          (* Write the new sub-state in the global automaton *)
-                          let new_loc := location <| sl_pte := Some (exploded_desc <|ged_state := SPS_STATE_PTE_INVALID_UNCLEAN (ai <| ai_lis := new_substate|>) |>)|> in
-                          let new_mem := ptc.(ptc_state) <| gsm_memory := <[location.(sl_phys_addr) := new_loc]> ptc.(ptc_state).(gsm_memory)|> in
-                          log (Mreturn new_mem)
-                      end
-                    else
-                      Mreturn ptc.(ptc_state)
-                  | _ => Mreturn ptc.(ptc_state)
+  | None => (* Cannot do anything if the page is not initialised *)
+    Merror (CME_uninitialised "tlbi_visitor" ptc.(ptc_addr))
+  | Some location =>
+    (* Test if there is something to do *)
+    match should_perform_tlbi td ptc with
+    | None => Merror CME_unimplemented
+    | Some b =>
+      if b then
+        (* step_pte_on_tlbi: inlined *)
+        match location.(sl_pte) with
+        | None => Merror (CME_internal_error IET_unexpected_none)
+          (* This cannot happen (otherwise, should_perform_tlbi would be false) *)
+        | Some exploded_desc =>
+          match exploded_desc.(ged_state) with
+          | SPS_STATE_PTE_INVALID_UNCLEAN ai =>
+            (* If the CPU that does the transformation is not the one that initiated the invalidation, do nothing *)
+            if bool_decide (cpu_id = ai.(ai_invalidator_tid)) then
+              let new_substate :=
+                (* Depending on the current state and the TLBI kind, we update the sub-state *)
+                match ai.(ai_lis) with
+                | LIS_dsbed => step_pte_on_tlbi_after_dsb td
+                | LIS_dsb_tlbi_ipa_dsb => step_pte_on_tlbi_after_tlbi_ipa td
+                | a => Some a (* Otherwise, it does not make the sub-automaton change *)
                 end
-            end
-          else (* In the case where the PTE is not affected by the TLBI, we do nothing *)
-            {|gsmsr_log := nil; gsmsr_data := Ok _ _ ptc.(ptc_state) |}
-      end
+              in
+              match new_substate with
+              | None => Merror CME_unimplemented
+              | Some new_substate =>
+                let log :=
+                  match new_substate, ai.(ai_lis) with
+                  | LIS_dsb_tlbied, LIS_dsbed => Mlog (Log "BBM: dsb'd->tlbied" (phys_addr_val ptc.(ptc_addr)))
+                  | LIS_dsb_tlbi_ipa, LIS_dsbed => Mlog (Log "BBM: dsb'd->tlbied_ipa" (phys_addr_val ptc.(ptc_addr)))
+                  | LIS_dsb_tlbied, LIS_dsb_tlbi_ipa_dsb => Mlog (Log "BBM: dsb_tlbi_ipa_dsbed->tlbied" (phys_addr_val ptc.(ptc_addr)))
+                  | _, _ => id
+                  end
+                in
+                (* Write the new sub-state in the global automaton *)
+                let new_loc := location <| sl_pte := Some (exploded_desc <|ged_state := SPS_STATE_PTE_INVALID_UNCLEAN (ai <| ai_lis := new_substate|>) |>)|> in
+                let new_mem := ptc.(ptc_state) <| cm_memory := <[location.(sl_phys_addr) := new_loc]> ptc.(ptc_state).(cm_memory)|> in
+                log (Mreturn new_mem)
+              end
+            else
+              Mreturn ptc.(ptc_state)
+          | _ => Mreturn ptc.(ptc_state)
+          end
+        end
+      else (* In the case where the PTE is not affected by the TLBI, we do nothing *)
+        {|cmr_log := nil; cmr_data := Ok _ _ ptc.(ptc_state) |}
+    end
   end
 .
 
-Definition step_tlbi (tid : thread_identifier) (td : TLBI) (gsm : casemate_model) : casemate_model_result :=
+Definition step_tlbi (tid : thread_identifier) (td : TLBI) (cm : casemate_model) : casemate_model_result :=
   match decode_tlbi td with
-  | None => Merror GSME_unimplemented
+  | None => Merror CME_unimplemented
   | Some decoded_TLBI =>
     match td.(TLBI_rec).(TLBIRecord_regime) with
     | Regime_EL2 =>
       (* traverse all s1 pages*)
-      traverse_si_pgt (Some tid) gsm (tlbi_visitor tid decoded_TLBI) S1
+      traverse_si_pgt (Some tid) cm (tlbi_visitor tid decoded_TLBI) S1
     | Regime_EL10 =>
       (* traverse s2 pages *)
-      traverse_si_pgt (Some tid) gsm (tlbi_visitor tid decoded_TLBI) S2
+      traverse_si_pgt (Some tid) cm (tlbi_visitor tid decoded_TLBI) S2
     | _ =>
       (* traverse all page tables and add a warning *)
-      let res := traverse_all_pgt (Some tid) gsm (tlbi_visitor tid decoded_TLBI) in
-      res <| gsmsr_log := Warning_unsupported_TLBI :: res.(gsmsr_log) |>
+      let res := traverse_all_pgt (Some tid) cm (tlbi_visitor tid decoded_TLBI) in
+      res <| cmr_log := Warning_unsupported_TLBI :: res.(cmr_log) |>
     end
   end
 .
@@ -708,8 +716,8 @@ Definition step_tlbi (tid : thread_identifier) (td : TLBI) (gsm : casemate_model
 
 Fixpoint si_root_exists (root : owner_t) (roots : list owner_t) : bool :=
   match roots with
-    | [] => false
-    | t :: q => (bool_decide (t = root)) || (si_root_exists root q)
+  | [] => false
+  | t :: q => (bool_decide (t = root)) || (si_root_exists root q)
   end
 .
 
@@ -721,52 +729,52 @@ Definition extract_si_root (val : u64) (stage : stage_t) : owner_t :=
 
 Definition register_si_root
   (tid : thread_identifier)
-  (gsm : casemate_model)
+  (cm : casemate_model)
   (root : owner_t)
   (stage : stage_t) :
   casemate_model_result :=
   let other_root_list :=
     match stage with
-      | S1 => pr_s2
-      | S2 => pr_s1
-    end gsm.(gsm_roots) in
+    | S1 => pr_s2
+    | S2 => pr_s1
+    end cm.(cm_roots) in
   (* Check that the root does not already exist in the other root list*)
-  if si_root_exists root other_root_list then Merror GSME_root_already_exists
+  if si_root_exists root other_root_list then Merror CME_root_already_exists
   else
     (* Add the root to the list of roots*)
     let new_roots :=
       match stage with
-        | S2 => gsm.(gsm_roots) <| pr_s2 := root :: gsm.(gsm_roots).(pr_s2) |>
-        | S1 => gsm.(gsm_roots) <| pr_s1 := root :: gsm.(gsm_roots).(pr_s1) |>
+      | S2 => cm.(cm_roots) <| pr_s2 := root :: cm.(cm_roots).(pr_s2) |>
+      | S1 => cm.(cm_roots) <| pr_s1 := root :: cm.(cm_roots).(pr_s1) |>
       end
     in
-    let new_st := gsm <| gsm_roots := new_roots |> in
+    let new_st := cm <| cm_roots := new_roots |> in
     (* then mark all its children as PTE *)
     match root with
-      | Root r => traverse_pgt_from root r pa0 l0 stage (mark_cb tid) new_st
+    | Root r => traverse_pgt_from root r pa0 l0 stage (mark_cb tid) new_st
     end
 .
 
-Definition step_msr (tid : thread_identifier) (md : trans_msr_data) (gsm : casemate_model) : casemate_model_result :=
+Definition step_msr (tid : thread_identifier) (md : trans_msr_data) (cm : casemate_model) : casemate_model_result :=
   let stage :=
     match md.(tmd_sysreg) with
-      | SYSREG_TTBR_EL2 => S1
-      | SYSREG_VTTBR => S2
+    | SYSREG_TTBR_EL2 => S1
+    | SYSREG_VTTBR => S2
     end
   in
   let root := extract_si_root md.(tmd_val) stage in
   (* The value written to TTRB is a root, it might be new. *)
   let roots :=
     match stage with
-      | S2 =>  pr_s2
-      | S1 => pr_s1
-    end gsm.(gsm_roots)
+    | S2 =>  pr_s2
+    | S1 => pr_s1
+    end cm.(cm_roots)
   in
-  if si_root_exists root (match stage with | S2 =>  pr_s2 | S1 => pr_s1 end gsm.(gsm_roots)) then
-    Mreturn gsm (* If it is already known to be a root, do nothing, it has already been registered *)
+  if si_root_exists root (match stage with | S2 =>  pr_s2 | S1 => pr_s1 end cm.(cm_roots)) then
+    Mreturn cm (* If it is already known to be a root, do nothing, it has already been registered *)
   else
     (* Otherwise, register it *)
-    register_si_root tid gsm root stage
+    register_si_root tid cm root stage
 .
 
 (** Hint *)
@@ -774,41 +782,41 @@ Definition step_msr (tid : thread_identifier) (md : trans_msr_data) (gsm : casem
 Definition step_hint_set_root_lock
   (root : owner_t)
   (addr : phys_addr_t)
-  (gsm : casemate_model) :
+  (cm : casemate_model) :
   casemate_model_result :=
-    Mreturn (gsm <| gsm_lock_addr := insert (phys_addr_val (root_val root)) (phys_addr_val addr) gsm.(gsm_lock_addr)|>)
+    Mreturn (cm <| cm_lock_addr := insert (phys_addr_val (root_val root)) (phys_addr_val addr) cm.(cm_lock_addr)|>)
 .
 
 Function set_owner_root
   (phys : phys_addr_t)
   (root : owner_t)
-  (gsm : casemate_model)
+  (cm : casemate_model)
   (logs : list log_element)
   (offs : Z)
   {measure Z.abs_nat offs} :
   casemate_model_result :=
   if Zle_bool offs 0 then
-    {| gsmsr_log := logs; gsmsr_data := Ok _ _ gsm |}
+    {| cmr_log := logs; cmr_data := Ok _ _ cm |}
   else
     let addr := phys pa+ (Phys_addr (bv_mul_Z_64 b8 (offs - 1))) in
-    match gsm !! addr with
-      | None =>
-        {|
-          gsmsr_log :=
-            logs;
-            gsmsr_data := Error _ _ (GSME_uninitialised "set_owner_root" addr)
-        |}
-      | Some location =>
-        let new_pte :=
-          match location.(sl_pte) with
-            | None => None
-            | Some pte => Some (pte <| ged_owner := root|>) (* actually change the root *)
-          end
-        in
-        (* Write the change to the global state *)
-        let new_loc := location <| sl_pte := new_pte |> in
-        let new_state := gsm <|gsm_memory := <[ location.(sl_phys_addr) := new_loc ]> gsm.(gsm_memory) |> in
-        set_owner_root phys root new_state logs (offs - 1)
+    match cm !! addr with
+    | None =>
+      {|
+        cmr_log :=
+          logs;
+          cmr_data := Error _ _ (CME_uninitialised "set_owner_root" addr)
+      |}
+    | Some location =>
+      let new_pte :=
+        match location.(sl_pte) with
+        | None => None
+        | Some pte => Some (pte <| ged_owner := root|>) (* actually change the root *)
+        end
+      in
+      (* Write the change to the global state *)
+      let new_loc := location <| sl_pte := new_pte |> in
+      let new_state := cm <|cm_memory := <[ location.(sl_phys_addr) := new_loc ]> cm.(cm_memory) |> in
+      set_owner_root phys root new_state logs (offs - 1)
     end
 .
 Set Warnings "-funind-cannot-build-inversion -funind-cannot-define-graph".
@@ -817,16 +825,16 @@ Set Warnings "funind-cannot-build-inversion funind-cannot-define-graph".
 
 Definition step_release_cb (ctx : page_table_context) : casemate_model_result :=
     match ctx.(ptc_loc) with
-    | None => Merror (GSME_uninitialised "step_release_cb"%string ctx.(ptc_addr))
+    | None => Merror (CME_uninitialised "step_release_cb"%string ctx.(ptc_addr))
     | Some location =>
       match location.(sl_pte) with
-        | None => Merror (GSME_not_a_pte "release_cb" ctx.(ptc_addr))
-        | Some desc =>
-          match desc.(ged_state) with
-            | SPS_STATE_PTE_INVALID_UNCLEAN _ =>
-                Merror (GSME_bbm_violation VT_release_unclean ctx.(ptc_addr))
-            | _ => Mreturn ctx.(ptc_state)
-          end
+      | None => Merror (CME_not_a_pte "release_cb" ctx.(ptc_addr))
+      | Some desc =>
+        match desc.(ged_state) with
+        | SPS_STATE_PTE_INVALID_UNCLEAN _ =>
+            Merror (CME_bbm_violation VT_release_unclean ctx.(ptc_addr))
+        | _ => Mreturn ctx.(ptc_state)
+        end
       end
   end
 .
@@ -834,96 +842,96 @@ Definition step_release_cb (ctx : page_table_context) : casemate_model_result :=
 
 Fixpoint remove (x : owner_t) (l : list owner_t) : list owner_t :=
   match l with
-    | nil => nil
-    | y::tl => if bool_decide (x = y) then remove x tl else y::(remove x tl)
+  | nil => nil
+  | y::tl => if bool_decide (x = y) then remove x tl else y::(remove x tl)
   end
 .
 
 Definition try_unregister_root
   (addr : owner_t)
   (cpu : thread_identifier)
-  (gsm : casemate_model) :
+  (cm : casemate_model) :
   casemate_model_result :=
-  match gsm !! root_val addr with
-    | None => Merror (GSME_internal_error IET_unexpected_none)
-    | Some loc =>
-      match loc.(sl_pte) with
-        | None => Merror (GSME_internal_error IET_unexpected_none)
-        | Some pte =>
-          let new_roots :=
-            match pte.(ged_stage) with
-              | S2 => gsm.(gsm_roots) <| pr_s2 := remove addr gsm.(gsm_roots).(pr_s2) |>
-              | S1 => gsm.(gsm_roots) <| pr_s1 := remove addr gsm.(gsm_roots).(pr_s1) |>
-            end
-          in
-          let gsm := gsm <| gsm_roots := new_roots |> in
-          traverse_pgt_from_root addr pte.(ged_stage) (unmark_cb cpu) gsm
-      end
+  match cm !! root_val addr with
+  | None => Merror (CME_internal_error IET_unexpected_none)
+  | Some loc =>
+    match loc.(sl_pte) with
+    | None => Merror (CME_internal_error IET_unexpected_none)
+    | Some pte =>
+      let new_roots :=
+        match pte.(ged_stage) with
+        | S2 => cm.(cm_roots) <| pr_s2 := remove addr cm.(cm_roots).(pr_s2) |>
+        | S1 => cm.(cm_roots) <| pr_s1 := remove addr cm.(cm_roots).(pr_s1) |>
+        end
+      in
+      let cm := cm <| cm_roots := new_roots |> in
+      traverse_pgt_from_root addr pte.(ged_stage) (unmark_cb cpu) cm
+    end
   end
 .
 
 Definition step_release_table
   (cpu : thread_identifier)
   (addr : owner_t)
-  (gsm : casemate_model) :
+  (cm : casemate_model) :
   casemate_model_result :=
-  match gsm !! root_val addr with
-    | None => Merror (GSME_uninitialised "release"%string (root_val addr))
-    | Some location =>
-      match location.(sl_pte) with
-        | None => Merror (GSME_not_a_pte "release"%string (root_val addr))
-        | Some desc =>
-          let new_st := traverse_pgt_from
-            addr
-            (root_val desc.(ged_owner))
-            desc.(ged_ia_region).(range_start)
-            desc.(ged_level)
-            desc.(ged_stage)
-            step_release_cb
-            gsm in
-          Mupdate_state (try_unregister_root (addr) cpu) new_st
-      end
+  match cm !! root_val addr with
+  | None => Merror (CME_uninitialised "release"%string (root_val addr))
+  | Some location =>
+    match location.(sl_pte) with
+    | None => Merror (CME_not_a_pte "release"%string (root_val addr))
+    | Some desc =>
+      let new_st := traverse_pgt_from
+        addr
+        (root_val desc.(ged_owner))
+        desc.(ged_ia_region).(range_start)
+        desc.(ged_level)
+        desc.(ged_stage)
+        step_release_cb
+        cm in
+      Mupdate_state (try_unregister_root (addr) cpu) new_st
+    end
   end
 .
 
 Definition step_hint_set_pte_thread_owner
   (phys : phys_addr_t)
   (val : owner_t)
-  (gsm : casemate_model) :
+  (cm : casemate_model) :
   casemate_model_result :=
-  match gsm !! phys with
-    | None => Merror (GSME_uninitialised "set_pte_thread_owner"%string phys)
-    | Some location =>
-      match location.(sl_pte) with
-        | None => Merror (GSME_not_a_pte "set_pte_thread_owner"%string phys)
-        | Some _ =>
-          let thread_owner := Thread_identifier (to_nat (phys_addr_val (root_val val))) in
-          Mreturn (gsm <| gsm_memory :=
-            (<[ location.(sl_phys_addr) := location <| sl_thread_owner := Some thread_owner |> ]> gsm.(gsm_memory))
-          |> )
-      end
+  match cm !! phys with
+  | None => Merror (CME_uninitialised "set_pte_thread_owner"%string phys)
+  | Some location =>
+    match location.(sl_pte) with
+    | None => Merror (CME_not_a_pte "set_pte_thread_owner"%string phys)
+    | Some _ =>
+      let thread_owner := Thread_identifier (to_nat (phys_addr_val (root_val val))) in
+      Mreturn (cm <| cm_memory :=
+        (<[ location.(sl_phys_addr) := location <| sl_thread_owner := Some thread_owner |> ]> cm.(cm_memory))
+      |> )
+    end
   end
 .
 
 Definition step_hint
   (cpu : thread_identifier)
   (hd : trans_hint_data)
-  (gsm : casemate_model)
+  (cm : casemate_model)
 : casemate_model_result :=
   match hd.(thd_hint_kind) with
-    | GHOST_HINT_SET_ROOT_LOCK =>
-      (* The types are weird here because of the order is reversed from SET_OWNER_ROOT (the root is first and the address second) *)
-      step_hint_set_root_lock (Root hd.(thd_location)) (root_val hd.(thd_value)) gsm
-      (* AFAIK, this only affects the internal locking discipline of the C simplified model and does nothing on the Coq version *)
-    | GHOST_HINT_SET_OWNER_ROOT =>
-      (* When ownership is transferred *)
-      (* Not sure about the size of the iteration *)
-      set_owner_root (align_4k hd.(thd_location)) hd.(thd_value) gsm [] z512
-    | GHOST_HINT_RELEASE =>
-      step_release_table cpu (Root hd.(thd_location)) gsm
-    | GHOST_HINT_SET_PTE_THREAD_OWNER =>
-      (* Set an owner thread of the PTE to track private ownership *)
-      step_hint_set_pte_thread_owner hd.(thd_location) hd.(thd_value) gsm
+  | GHOST_HINT_SET_ROOT_LOCK =>
+    (* The types are weird here because of the order is reversed from SET_OWNER_ROOT (the root is first and the address second) *)
+    step_hint_set_root_lock (Root hd.(thd_location)) (root_val hd.(thd_value)) cm
+    (* AFAIK, this only affects the internal locking discipline of the C simplified model and does nothing on the Coq version *)
+  | GHOST_HINT_SET_OWNER_ROOT =>
+    (* When ownership is transferred *)
+    (* Not sure about the size of the iteration *)
+    set_owner_root (align_4k hd.(thd_location)) hd.(thd_value) cm [] z512
+  | GHOST_HINT_RELEASE_TABLE =>
+    step_release_table cpu (Root hd.(thd_location)) cm
+  | GHOST_HINT_SET_PTE_THREAD_OWNER =>
+    (* Set an owner thread of the PTE to track private ownership *)
+    step_hint_set_pte_thread_owner hd.(thd_location) hd.(thd_value) cm
   end
 .
 
@@ -931,19 +939,28 @@ Definition step_hint
 Definition step_lock
   (cpu : thread_identifier)
   (hd : trans_lock_data)
-  (gsm : casemate_model)
+  (cm : casemate_model)
 : casemate_model_result :=
-  match hd.(tld_kind), lookup (phys_addr_val hd.(tld_addr)) gsm.(gsm_lock_state) with
-    | LOCK, None =>(* lock and authorize to write to that page-table *)
-        Mreturn (gsm <| gsm_lock_state := insert (phys_addr_val hd.(tld_addr)) cpu gsm.(gsm_lock_state) |>
-                    <| gsm_lock_authorization := insert (phys_addr_val hd.(tld_addr)) write_authorized gsm.(gsm_lock_authorization)|>)
-    | UNLOCK, Some thread =>
-      if bool_decide (thread = cpu) then
-        Mreturn (gsm <| gsm_lock_state := delete (phys_addr_val hd.(tld_addr)) gsm.(gsm_lock_state) |>)
-      else
-        Merror (GSME_double_lock_acquire cpu thread)
-    | LOCK, Some thread => Merror (GSME_double_lock_acquire cpu thread)
-    | UNLOCK, None => Merror (GSME_double_lock_acquire cpu cpu)
+  match lookup (phys_addr_val hd.(tld_addr)) cm.(cm_lock_state) with
+  | None =>(* lock and authorize to write to that page-table *)
+      Mreturn (cm <| cm_lock_state := insert (phys_addr_val hd.(tld_addr)) cpu cm.(cm_lock_state) |>
+                  <| cm_lock_authorization := insert (phys_addr_val hd.(tld_addr)) write_authorized cm.(cm_lock_authorization)|>)
+  | Some thread => Merror (CME_double_lock_acquire cpu thread)
+  end
+.
+
+Definition step_unlock
+  (cpu : thread_identifier)
+  (hd : trans_lock_data)
+  (cm : casemate_model)
+: casemate_model_result :=
+  match lookup (phys_addr_val hd.(tld_addr)) cm.(cm_lock_state) with
+  | Some thread =>
+    if bool_decide (thread = cpu) then
+      Mreturn (cm <| cm_lock_state := delete (phys_addr_val hd.(tld_addr)) cm.(cm_lock_state) |>)
+    else
+      Merror (CME_double_lock_acquire cpu thread)
+  | None => Merror (CME_double_lock_acquire cpu cpu)
   end
 .
 
